Let $\mathbf{O_1} = (x_1, y_1), \mathbf{O_2} = (x_2, y_2)$ be two centers of circles,  $r_1,r_2$ be the radius. If:\\
$ d = | \mathbf{O_1} - \mathbf{O_2} | $
$ \mathbf{u} = \frac{ 1 }{ 2 } ( \mathbf{O_1} + \mathbf{O_2} )+ 
\frac{ ( r_2^2 - r_1^2 )  }
{ 2 d^2 } ( \mathbf{O_1} - \mathbf{O_2} )$ \\
$ \mathbf{v} = \frac{ \sqrt{(r_1+r_2+d) (r_1-r_2+d) (r_1+r_2-d) (-r_1+r_2+d)} }{ 2 d^2 } ( y_1 - y_2 , -x_1 + x_2 )$
then $ \mathbf{u} + \mathbf{v} , \mathbf{u} - \mathbf{v} $
are the two intersections of the circles, provided that $ d < r_1 + r_2 $.

